# 公式汇总

----

## 双曲函数

  * 双曲正弦 $sh x = \frac{e^x - e^{(-x)}}{2}$
  * 双曲余弦 $ch x = \frac{e^x + e^{(-x)}}{2}$
  * 双曲正切 $th x = \frac{sh x}{ch x} = \frac{e^x - e^{(-x)}}{e^x + e^{(-x)}}$
  
  * 反双曲正弦 $arsh x = ln(x + \sqrt{x^2 + 1})$
  * 反双曲余弦 $arch x = ln(x + \sqrt{x^2 - 1})$
  * 反双曲正切 $arth x = \frac{1}{2} ln \frac{1+x}{1-x}$

推导公式：  
  * $sh(x + y) = sh x \cdot ch y + ch x \cdot sh y$
  * $sh(x - y) = sh x \cdot ch y - ch x \cdot sh y$
  * $ch(x + y) = ch x \cdot ch y + sh x \cdot sh y$
  * $ch(x - y) = ch x \cdot ch y - sh x \cdot sh y$

